refactor encoding proofs

theories/encoding.v
@@ -1,15 +1,11 @@
-From stdpp Require Import relations.
+From stdpp Require Import prelude.
 From Coq Require Import ssreflect.
-From ambig Require Import grammar decidability util ambiguity acyclic sub_derive.
+From ambig Require Import grammar util ambiguity acyclic sub_derive slice derivation witness.
 
 Section encoding.
 
-  Variable Σ N : Type.
-  Context `{!EqDecision Σ}.
-  Context `{!EqDecision N}.
-
-  Variable G : grammar Σ N.
-  Context `{!acyclic G}.
+  Context {Σ N : Type} `{EqDecision Σ} `{Inhabited Σ} `{EqDecision N}.
+  Context (G : grammar Σ N) `{acyclic G}.
 
   (* sat model *)
 
@@ -18,59 +14,154 @@ Section encoding.
     line : nat → nat;
     col : nat → nat;
     line_col i := (line i, col i);
-    can_derive : N → nat (* start (inclusive) *) → nat (* length *) → bool;
-    can_reach_from : N → nat (* start (inclusive) *) → nat (* length *) → bool;
+    can_derive : N → nat (* start (inclusive) *) → nat (* length, positive *) → bool;
+    can_reach_from : N → nat (* start (inclusive) *) → nat (* length, positive *) → bool;
+    ε_can_reach_from : N → bool;
   }.
 
-  Fixpoint decode m x δ : sentence Σ :=
-    match δ with
-    | 0 => []
-    | S n => term m x @ (line m x, col m x) :: decode m (S x) n
-    end.
+  (* decode *)
 
-  Lemma decode_length m x δ :
-    length (decode m x δ) = δ.
+  Definition decode m k : sentence Σ :=
+    (λ i, term m i @ (line m i, col m i)) <$> (index_range k).
+
+  Lemma decode_length m k :
+    length (decode m k) = k.
   Proof.
-    generalize dependent x.
-    induction δ => x //=.
-    naive_solver.
+    by rewrite fmap_length index_range_length.
   Qed.
 
-  Lemma decode_merge m x δ δ' :
-    decode m x δ ++ decode m (x + δ) δ' = decode m x (δ + δ').
+  Lemma decode_lookup m k i :
+    i < k → (decode m k) !! i = Some (term m i @ (line m i, col m i)).
   Proof.
-    generalize dependent x.
-    induction δ as [|n IHn] => x /=.
-    - by rewrite -plus_n_O.
-    - rewrite <- IHn.
-      have -> : x + S n = S x + n by lia.
-      done.
+    intros. rewrite list_lookup_fmap index_range_lookup //.
   Qed.
 
-  (* formula: a predicate over a model *)
+  (* encode *)
 
-  Definition formula : Type := model → Prop.
+  Global Instance acyclic_derive_dec A w :
+    Decision (G ⊨ A ⇒ w).
+  Admitted.
+
+  Global Instance acyclic_reachable_dec A w B h :
+    Decision (reachable G (A, w) (B, h)).
+  Admitted.
+
+  Definition encode S (w : sentence Σ) : model := {|
+    term i :=
+      match w !! i with
+      | Some (a @ _) => a
+      | None => inhabitant
+      end;
+    line i :=
+      match w !! i with
+      | Some (_ @ (x, _)) => x
+      | None => 0
+      end;
+    col i :=
+      match w !! i with
+      | Some (_ @ (_, y)) => y
+      | None => 0
+      end;
+    can_derive A x δ := bool_decide (G ⊨ A ⇒ slice w x δ);
+    can_reach_from A x δ := bool_decide (reachable G (S, w) (A, slice w x δ));
+    ε_can_reach_from A := bool_decide (reachable G (S, w) (A, []));
+  |}.
+
+  Lemma decode_encode S w :
+    decode (encode S w) (length w) = w.
+  Proof.
+    apply list_eq_same_length with (n := length w) => //.
+    1: by rewrite decode_length.
+    intros i x y ?. rewrite decode_lookup //=. repeat case_match.
+    - inversion 1; subst. intros Hy.
+      have Heq : Some (letter @ (n, n0)) = Some y by rewrite -Hy; symmetry.
+      by inversion Heq.
+    - rewrite Heqo. inversion 2.
+  Qed.
+
+  Implicit Type w : sentence Σ.
+  Implicit Type x δ : nat.
+  Context `{∀ w, NoDup w}.
+
+  (* formula: a predicate over a bounded model *)
+
+  Definition formula : Type := nat → model → Prop.
+
+  (* encoding predicate *)
+
+  Variable Φ_apply₁ : (unary_predicate Σ) → nat → nat → formula.
+  Variable Φ_apply₁_spec : ∀ φ x δ k m,
+    Φ_apply₁ φ x δ k m ↔ apply₁ φ (slice (decode m k) x δ) = true.
+
+  Variable Φ_apply₂ : (binary_predicate Σ) → nat → nat → nat → nat → formula.
+  Variable Φ_apply₂_spec : ∀ φ x1 δ1 x2 δ2 k m,
+    Φ_apply₂ φ x1 δ1 x2 δ2 k m ↔
+      apply₂ φ (slice (decode m k) x1 δ1) (slice (decode m k) x2 δ2) = true.
 
   (* encoding derivation *)
 
-  Definition Φ_derive k : formula := λ m,
+  Definition Φ_derive : formula := λ k m,
     ∀ A x δ, 0 < δ (* nonempty *) → x + δ ≤ k →
-      can_derive m A x δ = true ↔ Exists (λ α,
-        match α with
-        | ε => False (* not consider [] *)
-        | atom a => δ = 1 ∧ term m x = a
-        | unary B φ => apply₁ φ (decode m x δ) = true ∧ can_derive m B x δ = true
-        | binary Bl Br φ =>
+      can_derive m A x δ = true ↔ (
+        False ∨
+        (∃ a, A ↦ atom a ∈ G ∧ δ = 1 ∧ term m x = a) ∨
+        (∃ B φ, A ↦ unary B φ ∈ G ∧ Φ_apply₁ φ x δ k m ∧ can_derive m B x δ = true) ∨
+        (∃ Bl Br φ, A ↦ binary Bl Br φ ∈ G ∧ (
           (G ⊨ Bl ⇒ [] ∧ can_derive m Br x δ = true) ∨
           (G ⊨ Br ⇒ [] ∧ can_derive m Bl x δ = true) ∨
           (∃ δ', 0 < δ' < δ ∧
-            can_derive m Bl x δ' = true ∧
-            can_derive m Br (x + δ') (δ - δ') = true ∧
-            apply₂ φ (decode m x δ') (decode m (x + δ') (δ - δ')) = true)
-        end
-      ) (clauses G A).
+            can_derive m Bl x δ' = true ∧ can_derive m Br (x + δ') (δ - δ') = true ∧
+            Φ_apply₂ φ x δ' (x + δ') (δ - δ') k m)
+        ))
+      ).
 
-  Notation "⟨ x , y ⟩" := (existT x y).
+  Lemma Φ_derive_sat X w :
+    Φ_derive (length w) (encode X w).
+  Proof.
+    intros A x δ ? ?.
+    rewrite bool_decide_eq_true -derivation_spec -check_derive_spec.
+    unfold check_derive. setoid_rewrite derivation_spec.
+    simpl can_derive. setoid_rewrite bool_decide_eq_true.
+    setoid_rewrite Φ_apply₁_spec. setoid_rewrite Φ_apply₂_spec.
+    setoid_rewrite decode_encode.
+    repeat apply ZifyClasses.or_morph.
+    - rewrite slice_nil_iff; lia.
+    - setoid_rewrite slice_singleton_iff. split.
+      + intros [a [p [[? Hw] ?]]]. exists a. repeat split => //=. by rewrite Hw.
+      + intros [a [? [? Hw]]].
+        have [? Hx] : is_Some (w !! x) by apply lookup_lt_is_Some; lia.
+        simpl in Hw. rewrite Hx in Hw. case_match; subst.
+        exists a. eexists. repeat split; eauto.
+    - done.
+    - split.
+      + intros [Bl [Br [φ [? [w1 [w2 [Hw [Hφ [HBl HBr]]]]]]]]].
+        have Hl : length (w1 ++ w2) = δ.
+        { apply (f_equal length) in Hw. by rewrite slice_length in Hw. }
+        exists Bl, Br, φ. split; first done.
+        destruct w1 as [|tk1 w1]; last destruct w2.
+        * left. rewrite app_nil_l in Hw. by rewrite Hw.
+        * right; left. rewrite app_nil_r in Hw. by rewrite Hw.
+        * right; right. apply slice_app_inv_NoDup in Hw as [Hw1 Hw2] => //.
+          rewrite Hw1 in HBl, Hφ. rewrite Hw2 in HBr, Hφ.
+          rewrite app_length !cons_length in Hl.
+          exists (length (tk1 :: w1)). repeat split => //. all: rewrite cons_length; lia.
+      + intros [Bl [Br [φ [? [Hd|[Hd|Hd]]]]]].
+        * destruct Hd as [? ?].
+          exists Bl, Br, φ. split; first done.
+          exists [], (slice w x δ). rewrite app_nil_l.
+          repeat split => //. destruct φ as [φ Hφ]; apply Hφ; by left.
+        * destruct Hd as [? ?].
+          exists Bl, Br, φ. split; first done.
+          exists (slice w x δ), []. rewrite app_nil_r.
+          repeat split => //. destruct φ as [φ Hφ]; apply Hφ; by right.
+        * destruct Hd as [δ' [? [? [? ?]]]].
+          exists Bl, Br, φ. split; first done.
+          exists (slice w x δ'), (slice w (x + δ') (δ - δ')).
+          rewrite -slice_app. have -> : δ' + (δ - δ') = δ by lia.
+          repeat split => //.
+  Qed.
+
+  (* Notation "⟨ x , y ⟩" := (existT x y). *)
 
   Lemma list_nonempty_length {A} (l : list A) :
     l ≠ [] ↔ 0 < length l.
@@ -83,15 +174,15 @@ Section encoding.
      In this way, it suffices to show two propositions both using disjunction, but one is using
      `can_derive` and the other `_ ⊨ _ ⇒ _`, are equiv.
 
-     This approach will also simplifies the proof for `Φ_derive k (decode _ w)`, given that
+     This approach will also simplifies the proof for `Φ_derive k (model_slice _ w)`, given that
      all `can_derive` is defined as `bool_decide (_ ⊨ _ ⇒ _)`.
   *)
   Lemma Φ_derive_spec k m :
     Φ_derive k m →
     ∀ A x δ, 0 < δ → x + δ ≤ k →
-      can_derive m A x δ = true ↔ G ⊨ A ⇒ decode m x δ.
+      can_derive m A x δ = true ↔ G ⊨ A ⇒ slice (decode m k) x δ.
   Proof.
-    intros HΦ A x δ ? ?. rewrite -check_derive_spec.
+    intros HΦ A x δ ? ?.
     (* induction on range length *)
     generalize dependent A.
     generalize dependent x.
@@ -100,104 +191,183 @@ Section encoding.
     have Hwf : wf (flip (succ G)) by apply acyclic_succ_flip_wf.
     induction A as [A IHA] using (well_founded_induction Hwf).
     (* rewrite definition *)
-    rewrite HΦ; [|done..].
-    rewrite check_derive_equation big_or_true Exists_exists.
-    split.
-    - (* -> *)
-      intros [α [Hp Hα]]. exists ⟨α, Hp⟩.
-      case_match => //.
-      3: destruct Hα as [Hα|[Hα|Hα]].
-      + destruct Hα as [-> ?]. repeat case_match => //.
-        apply bool_decide_eq_true. naive_solver.
-      + destruct Hα as [? ?].
-        apply andb_true_iff. split => //.
-        clear IHδ. apply IHA => //. eapply succ_unary; eauto.
-      + destruct Hα as [Hn ?].
-        apply orb_true_iff; left. apply orb_true_iff; left.
-        apply when_true. exists Hn.
-        clear IHδ. apply IHA => //. eapply succ_right; eauto.
-      + destruct Hα as [Hn ?].
-        apply orb_true_iff; left. apply orb_true_iff; right.
-        apply when_true. exists Hn.
-        clear IHδ. apply IHA => //. eapply succ_left; eauto.
-      + destruct Hα as [δ' [? [? [? ?]]]].
-        apply orb_true_iff; right.
-        apply big_or_true.
-        have Hpar : (decode m x δ', decode m (x + δ') (δ - δ')) ∈ nonempty_partition (decode m x δ).
-        { eapply nonempty_partition_spec; eauto.
-          split. rewrite decode_merge. f_equal. lia.
-          split. all: apply list_nonempty_length.
-          all: rewrite decode_length; lia. }
-        exists ⟨(decode m x δ', decode m (x + δ') (δ - δ')), Hpar⟩.
-        apply andb_true_iff. split.
-        apply andb_true_iff. split => //.
-        all: clear IHA; apply IHδ; [lia..|done].
-      - (* <- *)
-        intros [[α Hp] Hα]. exists α. split; first by apply Hp.
-        case_match.
-        4: apply orb_true_iff in Hα as [Hα|Hα]; first apply orb_true_iff in Hα as [Hα|Hα].
-        + apply bool_decide_eq_true in Hα.
-          have ? : decode m x δ ≠ [].
-          { apply list_nonempty_length. rewrite decode_length. lia. }
-          contradiction.
-        + repeat case_match => //.
-          apply bool_decide_eq_true in Hα.
-          have ? : δ = 1.
-          { have Hl : length (decode m x δ) = 1 by rewrite Heqs.
-            by rewrite decode_length in Hl. }
-          subst. split => //. naive_solver.
-        + apply andb_true_iff in Hα as [? ?]. split => //.
-          clear IHδ. apply IHA => //. eapply succ_unary; eauto.
-        + apply when_true in Hα as [? ?]. left. split => //.
-          clear IHδ. apply IHA => //. eapply succ_right; eauto.
-        + apply when_true in Hα as [? ?]. right. left. split => //.
-          clear IHδ. apply IHA => //. eapply succ_left; eauto.
-        + apply big_or_true in Hα as [[[wl wr] Hw] Hα].
-          apply andb_true_iff in Hα as [Hα ?].
-          apply andb_true_iff in Hα as [? ?].
-          right. right.
-          eapply nonempty_partition_spec in Hw as [Hw [? ?]]; eauto.
-          exists (length wl).
-          have ? : length (decode m x δ) = δ by rewrite decode_length.
-          have ? : length (decode m x δ) = length wl + length wr
-            by rewrite Hw app_length.
-          have ? : 0 < length wl by apply list_nonempty_length.
-          have ? : 0 < length wr by apply list_nonempty_length.
-          have Hw' : decode m x δ = decode m x (length wl) ++
-            decode m (x + length wl) (δ - length wl).
-            by rewrite decode_merge; f_equal; lia.
-          have [Hwl Hwr] : decode m x (length wl) = wl ∧
-                           decode m (x + length wl) (δ - length wl) = wr.
-          { rewrite Hw in Hw'. apply app_inj_1 => //. by rewrite decode_length.  }
-          rewrite Hwl Hwr.
-          split; first lia. repeat split => //.
-          1,2: clear IHA; apply IHδ; [lia..|].
-          by rewrite Hwl. by rewrite Hwr.
-    (* TODO: why this is shelved? *)
-    Unshelve. done.
+    rewrite HΦ; [|done..]. setoid_rewrite Φ_apply₁_spec. setoid_rewrite Φ_apply₂_spec.
+    rewrite -derivation_spec -check_derive_spec /check_derive. setoid_rewrite derivation_spec.
+    repeat apply ZifyClasses.or_morph.
+    - rewrite slice_nil_iff ?decode_length; lia.
+    - setoid_rewrite slice_singleton_iff.
+      rewrite decode_lookup; first lia.
+      naive_solver.
+    - split.
+      + intros [B [φ [? [? ?]]]]. exists B, φ.
+        repeat split => //. apply IHA => //. eapply succ_unary; eauto.
+      + intros [B [φ [? [? ?]]]]. exists B, φ.
+        repeat split => //. apply IHA => //. eapply succ_unary; eauto.
+    - split.
+      + intros [Bl [Br [φ [? [Hd|[Hd|Hd]]]]]].
+        * destruct Hd as [? ?].
+          exists Bl, Br, φ. split; first done.
+          exists []. eexists. rewrite app_nil_l.
+          repeat split => //; first by destruct φ as [φ Hφ]; apply Hφ; by left.
+          apply IHA => //. eapply succ_right; eauto.
+        * destruct Hd as [? ?].
+          exists Bl, Br, φ. split; first done.
+          eexists. exists []. rewrite app_nil_r.
+          repeat split => //; first by destruct φ as [φ Hφ]; apply Hφ; by right.
+          apply IHA => //. eapply succ_left; eauto.
+        * destruct Hd as [δ' [? [? [? ?]]]].
+          exists Bl, Br, φ. split; first done.
+          do 2 eexists. repeat split; eauto.
+          1: by rewrite -slice_split.
+          all: apply IHδ => //; lia.
+      + intros [Bl [Br [φ [? [w1 [w2 [Hw [Hφ [HBl HBr]]]]]]]]].
+        have Hl : length (w1 ++ w2) = δ.
+        { apply (f_equal length) in Hw. rewrite slice_length in Hw; [rewrite decode_length; lia | done]. }
+        exists Bl, Br, φ. split; first done.
+        destruct w1 as [|tk1 w1]; last destruct w2.
+        * left. rewrite app_nil_l in Hw. split => //. 
+          apply IHA => //. eapply succ_right; eauto. by rewrite Hw.
+        * right; left. rewrite app_nil_r in Hw. split => //.
+          apply IHA => //. eapply succ_left; eauto. by rewrite Hw.
+        * right; right. apply slice_app_inv_NoDup in Hw as [Hw1 Hw2] => //.
+          rewrite Hw1 in HBl, Hφ. rewrite Hw2 in HBr, Hφ.
+          rewrite app_length !cons_length in Hl.
+          exists (length (tk1 :: w1)). repeat split => //.
+          3-4: apply IHδ => //.
+          all: rewrite cons_length; lia.
   Qed.
 
   (* encoding reachable from (S, [0..k]) *)
-  Definition Φ_reach k S : formula := λ m,
-    ∀ B x δ, (* δ can be zero *) x + δ ≤ k →
+  Definition Φ_reach_nonempty S : formula := λ k m,
+    ∀ B x δ, 0 < δ → x + δ ≤ k →
       can_reach_from m B x δ = true ↔ (
         (B = S ∧ x = 0 ∧ δ = k) ∨
-        (∃ A φ, A ↦ unary B φ ∈ G ∧ can_reach_from m A x δ = true ∧ apply₁ φ (decode m x δ) = true) ∨
+        (∃ A φ, A ↦ unary B φ ∈ G ∧ can_reach_from m A x δ = true ∧ Φ_apply₁ φ x δ k m) ∨
         (∃ A B' φ δ', x + δ + δ' ≤ k ∧ A ↦ binary B B' φ ∈ G ∧ can_reach_from m A x (δ + δ') = true ∧
           (if bool_decide (δ' = 0) then G ⊨ B' ⇒ [] else can_derive m B' (x + δ) δ' = true) ∧
-          apply₂ φ (decode m x δ) (decode m (x + δ) δ') = true) ∨
-        (∃ A B' φ δ', δ' ≤ x (* TODO *) ∧ A ↦ binary B' B φ ∈ G ∧ can_reach_from m A (x - δ') (δ' + δ) = true ∧
+          Φ_apply₂ φ x δ (x + δ) δ' k m) ∨
+        (∃ A B' φ δ', δ' ≤ x ∧ A ↦ binary B' B φ ∈ G ∧ can_reach_from m A (x - δ') (δ' + δ) = true ∧
           (if bool_decide (δ' = 0) then G ⊨ B' ⇒ [] else can_derive m B' (x - δ') δ' = true) ∧
-          apply₂ φ (decode m (x - δ') δ') (decode m x δ) = true)
+          Φ_apply₂ φ (x - δ') δ' x δ k m)
       ).
 
-  Lemma Φ_reach_spec k S m :
-    Φ_derive k m →
-    Φ_reach k S m →
-    ∀ B x δ, x + δ ≤ k →
-      can_reach_from m B x δ = true ↔ reachable G (S, decode m 0 k) (B, decode m x δ).
+  Definition Φ_reach_empty S : formula := λ k m,
+    ∀ B, ε_can_reach_from m B = true ↔ (
+      (B = S ∧ k = 0) ∨
+      (∃ A φ, A ↦ unary B φ ∈ G ∧ ε_can_reach_from m A = true) ∨
+      (∃ A B' φ, A ↦ binary B B' φ ∈ G ∧ (
+        (ε_can_reach_from m A = true ∧ G ⊨ B' ⇒ []) ∨
+        (∃ x δ, 0 < δ ∧ x + δ ≤ k ∧
+          can_reach_from m A x δ = true ∧ can_derive m B' x δ = true))) ∨
+      (∃ A B' φ, A ↦ binary B' B φ ∈ G ∧ (
+        (ε_can_reach_from m A = true ∧ G ⊨ B' ⇒ []) ∨
+        (∃ x δ, 0 < δ ∧ x + δ ≤ k ∧
+          can_reach_from m A x δ = true ∧ can_derive m B' x δ = true)))
+    ).
+
+  Definition Φ_reach S : formula := λ k m,
+    Φ_reach_nonempty S k m ∧ Φ_reach_empty S k m.
+
+  Lemma Φ_reach_nonempty_sat X w k :
+    length w = k →
+    Φ_reach_nonempty X k (encode X w).
   Proof.
-    intros HΦ' HΦ B x δ ?. rewrite -reachable_from_spec.
+    intros <- B x δ ? ?.
+    rewrite bool_decide_eq_true -reachable_from_spec -check_reachable_from_spec /=.
+    setoid_rewrite reachable_from_spec.
+    setoid_rewrite Φ_apply₁_spec. setoid_rewrite Φ_apply₂_spec.
+    setoid_rewrite decode_encode.
+    repeat apply ZifyClasses.or_morph.
+    - rewrite slice_full_iff; try lia. done. admit.
+    - by setoid_rewrite bool_decide_eq_true.
+    - split.
+      + intros [A [B' [φ [wr [? [Hr [? ?]]]]]]].
+        exists A, B', φ, (length wr).
+        rewrite bool_decide_eq_true. destruct wr as [|tk l].
+        * rewrite /= slice_nil ?Nat.add_0_r; [lia|].
+          rewrite app_nil_r in Hr.
+          repeat split => //.
+        * case_bool_decide => //. rewrite bool_decide_eq_true.
+          have Hsub : sublist (slice w x δ ++ tk :: l) w by eapply reachable_sublist; eauto.
+          apply sublist_slice in Hsub as [x' [? Hw']].
+          rewrite app_length slice_length in Hw'; [lia|]. symmetry in Hw'.
+          apply slice_app_inv_NoDup in Hw' as [Hwl Hwr] => //.
+          2: { apply list_nonempty_length. rewrite slice_length; lia. }
+          apply slice_eq_inv_NoDup in Hwl as [? _] => //.
+          2: { apply list_nonempty_length. lia. } subst.
+          rewrite slice_length in Hwr; first done.
+          have Htmp : δ + length (tk :: l) - δ = length (tk :: l) by lia.
+          rewrite Htmp in Hwr.
+          symmetry in Hwr. rewrite slice_app Hwr.
+          have HA : slice w (x + δ) (length (tk :: l)) ≠ [].
+          { rewrite Hwr. naive_solver. }
+          apply slice_nonempty_iff in HA.
+          repeat split => //. admit. admit.
+      + intros [A [B' [φ [δ' [? [? [Hr [Hd Hφ]]]]]]]].
+        apply bool_decide_eq_true in Hr.
+        exists A, B', φ, (slice w (x + δ) δ').
+        rewrite slice_app_merge_2.
+        repeat split => //.
+        case_bool_decide; [by subst | by apply bool_decide_eq_true in Hd].
+    - (* same as above *) admit.
+  Admitted.
+
+  Lemma apply_unary_nil (φ : unary_predicate Σ) :
+    apply₁ φ [] = true.
+  Proof. by destruct φ. Qed.
+
+  Lemma apply_binary_nil_l (φ : binary_predicate Σ) w :
+    apply₂ φ [] w = true.
+  Proof. destruct φ; naive_solver. Qed.
+
+  Lemma apply_binary_nil_r (φ : binary_predicate Σ) w :
+    apply₂ φ w [] = true.
+  Proof. destruct φ; naive_solver. Qed.
+
+  Lemma Φ_reach_empty_sat k X w :
+    length w = k →
+    Φ_reach_empty X k (encode X w).
+  Proof.
+    intros <- B.
+    rewrite bool_decide_eq_true -reachable_from_spec -check_reachable_from_spec /=.
+    setoid_rewrite reachable_from_spec.
+    setoid_rewrite bool_decide_eq_true.
+    repeat apply ZifyClasses.or_morph.
+    - rewrite length_zero_iff_nil. naive_solver.
+    - setoid_rewrite apply_unary_nil. naive_solver.
+    - setoid_rewrite apply_binary_nil_l. split.
+      + intros [A [B' [φ [w' [? [Hr [? ?]]]]]]].
+        exists A, B', φ. split; first done.
+        destruct w' as [|t w']; [by left | right].
+        have Hsub : sublist (t :: w') w by eapply reachable_sublist; eauto.
+        apply sublist_slice in Hsub as [a [? Hw]].
+        exists a, (length (t :: w')).
+        rewrite -Hw. repeat split => //. rewrite cons_length; lia.
+      + intros [A [B' [φ [? [Hr|Hr]]]]].
+        * destruct Hr as [? ?].
+          exists A, B', φ, [].
+          repeat split => //.
+        * destruct Hr as [x [δ [? [? [? ?]]]]].
+          exists A, B', φ, (slice w x δ).
+          repeat split => //.
+    - (* same as above *) admit.
+  Admitted.
+
+  Lemma Φ_reach_sat k X w :
+    length w = k →
+    Φ_reach X k (encode X w).
+  Proof.
+    intros <-. split; by [apply Φ_reach_nonempty_sat | apply Φ_reach_empty_sat].
+  Qed.
+
+  Lemma Φ_reach_nonempty_spec k S m :
+    Φ_derive k m →
+    Φ_reach_nonempty S k m →
+    ∀ B x δ, 0 < δ → x + δ ≤ k →
+      can_reach_from m B x δ = true → (* only this direction is needed *)
+      reachable G (S, decode m k) (B, slice (decode m k) x δ).
+  Proof.
+    intros HΦ' HΦ B x δ ? ? ?. rewrite -reachable_from_spec.
     (* induction on range length *)
     generalize dependent B.
     generalize dependent x.
@@ -206,218 +376,173 @@ Section encoding.
     (* induction on nonterminal *)
     have Hwf : wf (succ G) by apply acyclic_succ_wf.
     induction B as [B IHB] using (well_founded_induction Hwf).
-    rewrite HΦ; last done.
-    split.
-    - (* -> *) 
-      intros [Hr|[Hr|[Hr|Hr]]].
-      + destruct Hr as [-> [-> ->]]. apply reachable_from_refl.
-      + destruct Hr as [A [φ [? [? ?]]]].
-        eapply reachable_from_unary; eauto.
-        apply IHB => //. eapply succ_unary; eauto.
-      + destruct Hr as [A [B' [φ [δ' [? [? [? [? ?]]]]]]]].
-        case_bool_decide; subst.
-        * eapply reachable_from_left; eauto.
-          rewrite app_nil_r. apply IHB; last naive_solver.
-          eapply succ_left; eauto.
-        * eapply reachable_from_left; eauto.
-          2: eapply Φ_derive_spec; eauto; lia.
-          rewrite decode_merge. apply IHδ => //; lia.
-      + destruct Hr as [A [B' [φ [δ' [? [? [Hr [? ?]]]]]]]].
-        case_bool_decide; subst; eapply reachable_from_right; eauto.
-        * rewrite Nat.sub_0_r Nat.add_0_l in Hr. rewrite app_nil_l.
-          apply IHB => //. eapply succ_right; eauto.
-        * have Hx : x = x - δ' + δ' by lia.
-          rewrite {2}Hx decode_merge. apply IHδ => //; lia.
-        * eapply Φ_derive_spec; eauto; lia.
-    - (* <- *)
-      inversion 1; subst.
-      + left.
-        have Hl : length (decode m 0 k) = length (decode m x δ) by congruence.
-        rewrite !decode_length in Hl.
-        split => //. lia.
-      + right; left.
-        exists A, φ. repeat split => //.
-        apply IHB => //. eapply succ_unary; eauto.
-      + right; right; left.
-        have H3' := H3.
-        apply reachable_from_spec, reachable_sublist in H3 => //.
-        have Hw2 : w2 = decode m (x + δ) (length w2). admit.
-        have Hw2l : x + δ + length w2 ≤ k. admit.
-        exists A, Br, φ, (length w2). repeat split => //.
-        * destruct w2 => /=.
-          rewrite app_nil_r in H3'. rewrite Nat.add_0_r. apply IHB => //.
-          eapply succ_left; eauto.
-          rewrite cons_length in Hw2. rewrite cons_length in Hw2l.
-          apply IHδ; [lia.. | by rewrite -decode_merge -Hw2].
-        * destruct w2 => //=.
-          eapply Φ_derive_spec; eauto. lia.
-          rewrite cons_length in Hw2. by rewrite -Hw2.
-        * by rewrite -Hw2.
-      + right; right; right.
-        have H3' := H3.
-        apply reachable_from_spec, reachable_sublist in H3 => //.
-        have Hw1 : w1 = decode m (x - length w1) (length w1). admit.
-        have Hw1l : length w1 ≤ x. admit.
-        exists A, Bl, φ, (length w1). repeat split => //.
-        * destruct w1 => /=.
-          rewrite app_nil_l in H3'. rewrite Nat.sub_0_r. apply IHB => //.
-          eapply succ_right; eauto.
-          rewrite cons_length in Hw1. rewrite cons_length in Hw1l.
-          apply IHδ; [lia.. | ].
-          have -> : Datatypes.S (length w1 + δ) = (Datatypes.S (length w1)) + δ by lia.
-          rewrite -decode_merge Nat.sub_add //.
-          by rewrite Hw1 in H3'.
-        * destruct w1 => //=.
-          eapply Φ_derive_spec; eauto. lia.
-          rewrite Nat.sub_add //. lia.
-          rewrite cons_length in Hw1. by rewrite -Hw1.
-        * by rewrite -Hw1.
-    Admitted.
+    rewrite HΦ //.
+    setoid_rewrite Φ_apply₁_spec. setoid_rewrite Φ_apply₂_spec.
+    intros [Hr|[Hr|[Hr|Hr]]].
+    - destruct Hr as [-> [-> ->]].
+      rewrite slice_full ?decode_length //.
+      constructor.
+    - destruct Hr as [A [φ [? [? ?]]]].
+      eapply reachable_from_unary; eauto.
+      apply IHB => //. eapply succ_unary; eauto.
+    - destruct Hr as [A [B' [φ [δ' [? [? [? [? ?]]]]]]]].
+      case_bool_decide; subst.
+      * eapply reachable_from_left; eauto.
+        rewrite app_nil_r. apply IHB; last naive_solver.
+        eapply succ_left; eauto.
+      * eapply reachable_from_left; eauto.
+        2: eapply Φ_derive_spec; eauto; lia.
+        rewrite slice_app_merge_2. apply IHδ => //; lia.
+    - destruct Hr as [A [B' [φ [δ' [? [? [Hr [? ?]]]]]]]].
+      case_bool_decide; subst; eapply reachable_from_right; eauto.
+      * rewrite Nat.sub_0_r Nat.add_0_l in Hr. rewrite app_nil_l.
+        apply IHB => //. eapply succ_right; eauto.
+      * rewrite slice_merge_2. apply IHδ => //; lia.
+      * eapply Φ_derive_spec; eauto; lia.
+  Qed.
 
-  (* decode properties *)
-
-  Lemma decode_empty m x δ :
-    decode m x δ = [] ↔ δ = 0.
+  Lemma Φ_reach_empty_spec S k m :
+    Φ_derive k m →
+    Φ_reach_nonempty S k m →
+    Φ_reach_empty S k m →
+    ∀ B,
+      ε_can_reach_from m B = true → (* only this direction is needed *)
+      reachable G (S, decode m k) (B, []).
   Proof.
-    (* intros H. *)
-    (* have : length (decode m x δ) = length [] by rewrite H. *)
-    (* rewrite decode_length. naive_solver. *)
-  Admitted.
+    intros ? ? HΦ B. rewrite -reachable_from_spec.
+    (* induction on nonterminal *)
+    have Hwf : wf (succ G) by apply acyclic_succ_wf.
+    induction B as [B IHB] using (well_founded_induction Hwf).
+    rewrite HΦ //. intros [Hr|[Hr|[Hr|Hr]]].
+      + destruct Hr as [<- ->]. constructor.
+      + destruct Hr as [A [φ [Hp ?]]].
+        eapply reachable_from_unary; [apply Hp | | apply apply_unary_nil].
+        apply IHB => //. eapply succ_unary; eauto.
+      + destruct Hr as [A [B' [φ [Hp [Hr|Hr]]]]].
+        * destruct Hr as [? ?].
+          eapply reachable_from_left; [apply Hp | | eauto | apply apply_binary_nil_l].
+          rewrite app_nil_l. apply IHB => //. eapply succ_left; eauto.
+        * destruct Hr as [x [δ [? [? [Hr Hd]]]]].
+          eapply Φ_derive_spec in Hd; eauto.
+          eapply reachable_from_left; [apply Hp | | eauto | apply apply_binary_nil_l].
+          rewrite app_nil_l. apply reachable_from_spec, Φ_reach_nonempty_spec; eauto.
+      + destruct Hr as [A [B' [φ [Hp [Hr|Hr]]]]].
+        * destruct Hr as [? ?].
+          eapply reachable_from_right; [apply Hp | | eauto | apply apply_binary_nil_r].
+          rewrite app_nil_r. apply IHB => //. eapply succ_right; eauto.
+        * destruct Hr as [x [δ [? [? [Hr Hd]]]]].
+          eapply Φ_derive_spec in Hd; eauto.
+          eapply reachable_from_right; [apply Hp | | eauto | apply apply_binary_nil_r].
+          rewrite app_nil_r. apply reachable_from_spec, Φ_reach_nonempty_spec; eauto.
+  Qed.
 
-  Lemma decode_singleton m x δ a p :
-    decode m x δ = [a @ p] →
-    δ = 1 ∧ a = term m x ∧ p = (line m x, col m x).
-  Proof.
-    intros H.
-  Admitted.
+  (* encoding derivations using different productions *)
 
-  Lemma decode_app_l m x δ w1 w2 :
-    decode m x δ = w1 ++ w2 →
-    decode m x (length w1) = w1.
-  Admitted.
-
-  (* encoding derivations of different prologue *)
-
-  Inductive prologue : Type :=
-  | pro_ε
-  | pro_atom (a : Σ)
-  | pro_unary (A : N)
-  | pro_binary (A B : N) (δ : nat) (* length of first part *)
+  Inductive using_clause : Type :=
+  | using_ε : using_clause
+  | using_atom : Σ → using_clause
+  | using_unary : N → unary_predicate Σ → using_clause
+  | using_binary : N → N → binary_predicate Σ → nat (* length of first part *) → using_clause
   .
 
-  Local Instance prologue_elem_of_nonterm : ElemOf prologue N := λ ψ A,
-    match ψ with
-    | pro_ε => A ↦ ε ∈ G
-    | pro_atom a => A ↦ atom a ∈ G
-    | pro_unary B => ∃ φ, A ↦ unary B φ ∈ G
-    | pro_binary Bl Br _ => ∃ φ, A ↦ binary Bl Br φ ∈ G
+  Definition usable_clauses A δ : list using_clause :=
+    flat_map (λ α, match α with
+    | ε => [using_ε]
+    | atom a => [using_atom a]
+    | unary B φ => [using_unary B φ]
+    | binary Bl Br φ => (λ δ', using_binary Bl Br φ δ') <$> (index_range δ ++ [δ])
+    end) (clauses G A).
+
+  Lemma elem_of_usable_clauses ψ A δ :
+    ψ ∈ usable_clauses A δ ↔ match ψ with
+    | using_ε => A ↦ ε ∈ G
+    | using_atom a => A ↦ atom a ∈ G
+    | using_unary B φ => A ↦ unary B φ ∈ G
+    | using_binary Bl Br φ δ' => A ↦ binary Bl Br φ ∈ G ∧ δ' ≤ δ
     end.
-
-  Definition Φ_pro ψ A x δ : formula := λ m,
-    match ψ with
-    | pro_ε => δ = 0
-    | pro_atom a => δ = 1 ∧ a = term m x
-    | pro_unary B =>
-      match δ with
-      | 0 => G ⊨ B ⇒ []
-      | _ => can_derive m B x δ = true ∧
-        apply₁ (unary_clause_predicate _ _ G A B) (decode m x δ) = true
-      end
-    | pro_binary Bl Br δ' =>
-      match δ', δ - δ' with
-      | 0, _ => G ⊨ Bl ⇒ [] ∧ can_derive m Br x δ = true
-      | _, 0 => can_derive m Bl x δ' = true ∧ G ⊨ Br ⇒ []
-      | _, _ => can_derive m Bl x δ' = true ∧ 
-        can_derive m Br (x + δ') (δ - δ') = true ∧
-        apply₂ (binary_clause_predicate _ _ G A Bl Br) (decode m x δ') (decode m (x + δ') (δ - δ')) = true
-      end
-    end.
-
-  (* Definition Φ_binary_derive Bl Br φ x δl δr : formula := λ m,
-    match δl, δr with
-    | 0, _ => G ⊨ Bl ⇒ [] ∧ can_derive m Br x δr = true
-    | _, 0 => can_derive m Bl x δl = true ∧ G ⊨ Br ⇒ []
-    | _, _ => can_derive m Bl x δl = true ∧ can_derive m Br (x + δl) δr = true ∧
-      apply₂ φ (decode m x δl) (decode m (x + δl) δr) = true
-    end.
-
-  Lemma Φ_binary_derive_witness k m x δl δr A Bl Br φ :
-    Φ_derive k m →
-    x + δl + δr ≤ k →
-    A ↦ binary Bl Br φ ∈ G →
-    Φ_binary_derive Bl Br φ x δl δr m ↔
-      ∃ t1 t2, root t1 = Bl ∧ root t2 = Br ∧ word t1 = decode m x δl ∧
-        (binary_tree A t1 t2) ▷ A ={G}=> decode m x (δl + δr). *)
-  (* Proof.
-    intros ? ? ? ? ? [Hdl [Hdr ?]].
-    eapply Φ_derive_spec in Hdl as [t1 [? [? ?]]]; eauto; try lia.
-    eapply Φ_derive_spec in Hdr as [t2 [? [? ?]]]; eauto; try lia.
-    exists t1, t2. repeat split => //.
-    have ? : decode m x δ' ++ decode m (x + δ') (δ - δ') = decode m x δ.
-    { rewrite decode_merge. by have -> : δ' + (δ - δ') = δ by lia. }
-    repeat split. simpl in *. congruence.
-    econstructor => //. naive_solver. by rewrite H9 H6.
-  Qed. *)
-(* 
-  Definition Φ_clause_derive (α : clause Σ N) (x δ : nat) : formula := λ m,
-    match α with
-    | ε => δ = 0
-    | atom a => δ = 1 ∧ term m x = a
-    | unary A φ =>
-      match δ with
-      | 0 => G ⊨ A ⇒ []
-      | _ => can_derive m A x δ = true ∧ apply₁ φ (decode m x δ) = true
-      end
-    | binary Bl Br φ => ∃ δl δr,
-      δl + δr = δ ∧ Φ_binary_derive Bl Br φ x δl δr m
-    end. *)
-
-  Ltac solve_witness :=
-    repeat split; simpl; try done; try congruence;
-    econstructor; eauto.
-
-  Lemma Φ_pro_witness k m x δ A ψ :
-    Φ_derive k m →
-    x + δ ≤ k →
-    ψ ∈ A →
-    Φ_pro ψ A x δ m ↔ match ψ with
-      | pro_ε => δ = 0 ∧ ε_tree A ▷ A ={G}=> decode m x δ
-      | pro_atom a => δ = 1 ∧ a = term m x ∧ let p := (line m x, col m x) in
-        (token_tree A (a @ p)) ▷ A ={G}=> decode m x δ
-      | pro_unary B => ∃ t, root t = B ∧ (unary_tree A t) ▷ A ={G}=> decode m x δ
-      | pro_binary Bl Br δ' => ∃ t1 t2, root t1 = Bl ∧ root t2 = Br ∧
-        word t1 = decode m x δ' ∧ (binary_tree A t1 t2) ▷ A ={G}=> decode m x δ
-      end.
-  Proof.
-    intros ? ? Hψ. case_match => /=; split.
-    all: simpl in Hψ.
-    - intros ->. solve_witness.
-    - naive_solver.
-    - intros [-> ->]. solve_witness.
-    - naive_solver.
-    - destruct Hψ as [φ ?].
-      case_match.
-      * intros [t [? [? ?]]]. subst. exists t. solve_witness.
-        destruct φ as [φ ?]. simpl. congruence.
-      * intros [? ?].
-        eapply Φ_derive_spec in H2 as [t [? [? ?]]]; eauto; try lia.
-        subst. exists t. solve_witness.
-        have ? : unary_clause_predicate Σ N G A (root t) = φ. admit.
-        congruence.
-    - destruct Hψ as [φ ?].
-      intros [t [? [? [? Ht]]]]. inversion Ht; subst; clear Ht.
-      case_match. 2: split.
-      * exists t. solve_witness.
-      * eapply Φ_derive_spec; eauto; try lia. exists t. solve_witness.
-      * have ? : word (unary_tree A t) = word t by done.
-        have ? : unary_clause_predicate Σ N G A (root t) = φ0. admit.
-        congruence.
-    - destruct Hψ as [φ ?]. repeat case_match.
   Admitted.
 
-  Definition Φ_multi (A : N) (x δ : nat) : formula := λ m,
-    ∃ ψ1, ψ1 ∈ A ∧
-     ∃ ψ2, ψ2 ∈ A ∧ ψ1 ≠ ψ2 ∧ Φ_pro ψ1 A x δ m ∧ Φ_pro ψ2 A x δ m.
+  Definition Φ_using_derive ψ x δ : formula :=
+    match ψ with
+    | using_ε => λ k m, δ = 0
+    | using_atom a => λ k m, δ = 1 ∧ term m x = a
+    | using_unary B φ => λ k m,
+      if bool_decide (δ = 0) then G ⊨ B ⇒ []
+      else Φ_apply₁ φ x δ k m ∧ can_derive m B x δ = true
+    | using_binary Bl Br φ δ' => λ k m,
+      (if bool_decide (δ' = 0) then G ⊨ Bl ⇒ [] else can_derive m Bl x δ' = true) ∧
+      (if bool_decide (δ - δ' = 0) then G ⊨ Br ⇒ [] else can_derive m Br (x + δ') (δ - δ') = true) ∧
+      Φ_apply₂ φ x δ' (x + δ') (δ - δ') k m
+    end.
+
+  Lemma Φ_using_derive_witness k m x δ A ψ :
+    Φ_derive k m →
+    x + δ ≤ k →
+    ψ ∈ usable_clauses A δ →
+    Φ_using_derive ψ x δ k m ↔ match ψ with
+    | using_ε => δ = 0 ∧ ε_tree A ▷ A ={G}=> slice (decode m k) x δ
+    | using_atom a => δ = 1 ∧ a = term m x ∧ let p := (line m x, col m x) in
+      (token_tree A (a @ p)) ▷ A ={G}=> slice (decode m k) x δ
+    | using_unary B _ => ∃ t, root t = B ∧ (unary_tree A t) ▷ A ={G}=> slice (decode m k) x δ
+    | using_binary Bl Br _ δ' => ∃ t1 t2, root t1 = Bl ∧ root t2 = Br ∧
+      word t1 = slice (decode m k) x δ' ∧ (binary_tree A t1 t2) ▷ A ={G}=> slice (decode m k) x δ
+    end.
+  Proof.
+    intros ? ? Hψ. destruct ψ as [| a | B φ | Bl Br φ δ'] => /=.
+    all: apply elem_of_usable_clauses in Hψ.
+    - split; last naive_solver.
+      intros ->. split; first done. by apply witness_ε.
+    - split; last naive_solver.
+      intros [-> Hx]. split; first done.
+      erewrite slice_singleton; last by rewrite decode_lookup; [lia|eauto].
+      rewrite Hx. split; first done. by apply witness_atom.
+    - unfold derive. case_bool_decide.
+      + subst. rewrite slice_nil ?decode_length; [lia|].
+        split.
+        * intros [t [? [? ?]]]. exists t.
+          rewrite witness_unary; eauto. repeat split => //. apply apply_unary_nil.
+        * intros [t [? Ht]]. eapply witness_unary in Ht; eauto. naive_solver.
+      + rewrite Φ_apply₁_spec.
+        rewrite Φ_derive_spec; eauto; [|lia]. unfold derive.
+        split.
+        * intros [? [t [? [? ?]]]]. exists t.
+          rewrite witness_unary; eauto. repeat split => //.
+        * intros [t [? Ht]]. eapply witness_unary in Ht; eauto. naive_solver.
+    - destruct Hψ as [Hψ ?]. unfold derive. rewrite Φ_apply₂_spec. repeat case_bool_decide.
+      + have -> : δ = 0 by lia.
+        have -> : slice (decode m k) x 0 = [] ++ [] by rewrite slice_nil ?decode_length; [lia|].
+        have -> : δ' = 0 by lia. rewrite slice_nil ?decode_length; [lia|].
+        split.
+        * intros [[t1 [? [? ?]]] [[t2 [? [? ?]]] ?]]. exists t1, t2.
+          rewrite witness_binary; eauto. repeat split => //.
+        * intros [t1 [t2 [? [? [? Ht]]]]]. eapply witness_binary in Ht; eauto. naive_solver.
+      + have -> : slice (decode m k) x δ = [] ++ slice (decode m k) x δ by rewrite app_nil_l.
+        subst. rewrite Nat.add_0_r Nat.sub_0_r slice_nil ?decode_length; [lia|].
+        rewrite Φ_derive_spec; eauto; [|lia]. unfold derive.
+        split.
+        * intros [[t1 [? [? ?]]] [[t2 [? [? ?]]] ?]]. exists t1, t2.
+          rewrite witness_binary; eauto. repeat split => //.
+        * intros [t1 [t2 [? [? [? Ht]]]]]. eapply witness_binary in Ht; eauto. naive_solver.
+      + have -> : slice (decode m k) x δ = slice (decode m k) x δ ++ [] by rewrite app_nil_r.
+        have -> : δ' = δ by lia. rewrite Nat.sub_diag slice_nil ?decode_length; [lia|].
+        rewrite Φ_derive_spec; eauto; [|lia]. unfold derive.
+        split.
+        * intros [[t1 [? [? ?]]] [[t2 [? [? ?]]] ?]]. exists t1, t2.
+          rewrite witness_binary; eauto. repeat split => //.
+        * intros [t1 [t2 [? [? [? Ht]]]]]. eapply witness_binary in Ht; eauto. naive_solver.
+      + have -> : slice (decode m k) x δ = slice (decode m k) x δ' ++ slice (decode m k) (x + δ') (δ - δ')
+          by rewrite -slice_split.
+        rewrite !Φ_derive_spec; eauto; [|lia..]. unfold derive.
+        split.
+        * intros [[t1 [? [? ?]]] [[t2 [? [? ?]]] ?]]. exists t1, t2.
+          rewrite witness_binary; eauto. repeat split => //.
+        * intros [t1 [t2 [? [? [? Ht]]]]]. eapply witness_binary in Ht; eauto. naive_solver.
+  Qed.
+
+  Definition Φ_multi_usable (A : N) (x δ : nat) : formula := λ k m,
+    ∃ ψ1, ψ1 ∈ usable_clauses A δ ∧
+      ∃ ψ2, ψ2 ∈ usable_clauses A δ ∧
+        ψ1 ≠ ψ2 ∧ Φ_using_derive ψ1 x δ k m ∧ Φ_using_derive ψ2 x δ k m.
 
   Lemma wrap_with_id (P : Prop) :
     P ↔ id P.
@@ -425,18 +550,24 @@ Section encoding.
 
   Ltac wrap H := apply ->wrap_with_id in H.
 
-  Lemma Φ_multi_spec k m x δ A :
+  Lemma app_length_le_l {A} (l1 l2 l : list A) :
+    l1 ++ l2 = l →
+    length l1 ≤ length l.
+  Admitted.
+
+  Lemma Φ_multi_usable_spec k m x δ A :
     Φ_derive k m →
     x + δ ≤ k →
-    Φ_multi A x δ m ↔ ∃ t1, t1 ▷ A ={G}=> decode m x δ ∧
-      ∃ t2, t2 ▷ A ={G}=> decode m x δ ∧ ¬ similar t1 t2.
+    Φ_multi_usable A x δ k m ↔ ∃ t1, t1 ▷ A ={G}=> slice (decode m k) x δ ∧
+      ∃ t2, t2 ▷ A ={G}=> slice (decode m k) x δ ∧ ¬ similar t1 t2.
   Proof.
     intros ? ?. split.
     - (* -> *)
-      intros [ψ1 [ψ2 [? [? [? [Hψ1 Hψ2]]]]]].
-      eapply Φ_pro_witness in Hψ1; eauto.
-      eapply Φ_pro_witness in Hψ2; eauto.
+      intros [ψ1 [Hψ1 [ψ2 [Hψ2 [Hne [HΦ1 HΦ2]]]]]].
+      eapply Φ_using_derive_witness in HΦ1; eauto.
+      eapply Φ_using_derive_witness in HΦ2; eauto.
       repeat case_match.
+      all: apply elem_of_usable_clauses in Hψ1, Hψ2.
       all: repeat match goal with
       | [ H : _ ∧ _ |- _ ] => destruct H as [? ?]
       | [ H : ∃ _, _ |- _ ] => destruct H as [? ?]
@@ -446,32 +577,30 @@ Section encoding.
       | [ H : ?t ▷ ?A ={?G}=> ?w |- ∃ t, t ▷ ?A ={?G}=> ?w ∧ _ ] =>
         exists t; split; [by apply H|]; clear H
       end => //.
-      + congruence. 
-      + simpl. intros [? [? ?]]; subst.
-        have Hl : length (decode m x δ1) = length (decode m x δ0)
-          by f_equal; congruence.
-        rewrite !decode_length in Hl. congruence.
+      admit. admit.
     - (* <- *)
       intros [t1 [[? [? Ht1]] [t2 [[? [? Ht2]] ?]]]].
       destruct t1; destruct t2.
       all: simpl in *; try done; try congruence.
       all: inversion Ht1; subst; clear Ht1.
       all: inversion Ht2; subst; clear Ht2.
-      all: unfold Φ_multi.
+      all: unfold Φ_multi_usable.
       all: repeat match goal with
-      | [ H : ?A ↦ ε ∈ _ |- ∃ ψ, ψ ∈ ?A ∧ _ ] =>
-        assert (pro_ε ∈ A) by (apply H);
-        exists pro_ε; split; [done|]; wrap H
-      | [ H : ?A ↦ atom ?a ∈ _ |- ∃ ψ, ψ ∈ ?A ∧ _ ] =>
-        assert (pro_atom a ∈ A) by (apply H);
-        exists (pro_atom a); split; [done|]; wrap H
-      | [ H : ?A ↦ unary ?B ?φ ∈ _ |- ∃ ψ, ψ ∈ ?A ∧ _ ] =>
-        assert (pro_unary B ∈ A) by (by exists φ);
-        exists (pro_unary B); split; [done|]; wrap H
-      | [ H : ?A ↦ binary (root ?t1) (root ?t2) ?φ ∈ _ |- ∃ ψ, ψ ∈ ?A ∧ _ ] =>
-        assert (pro_binary (root t1) (root t2) (length (word t1)) ∈ A) by (by exists φ);
-        exists (pro_binary (root t1) (root t2) (length (word t1)));
-        split; [done|]; wrap H
+      | [ H : ?A ↦ ε ∈ _ |- ∃ ψ, ψ ∈ usable_clauses ?A ?δ ∧ _ ] =>
+        assert (using_ε ∈ usable_clauses A δ) by (by apply elem_of_usable_clauses);
+        eexists; split; [eauto|]; wrap H
+      | [ H : ?A ↦ atom ?a ∈ _ |- ∃ ψ, ψ ∈ usable_clauses ?A ?δ ∧ _ ] =>
+        assert (using_atom a ∈ usable_clauses A δ) by (by apply elem_of_usable_clauses);
+        eexists; split; [eauto|]; wrap H
+      | [ H : ?A ↦ unary ?B ?φ ∈ _ |- ∃ ψ, ψ ∈ usable_clauses ?A ?δ ∧ _ ] =>
+        assert (using_unary B φ ∈ usable_clauses A δ) by (by apply elem_of_usable_clauses);
+        eexists; split; [eauto|]; wrap H
+      | [ H : ?A ↦ binary (root ?t1) (root ?t2) ?φ ∈ _ |- ∃ ψ, ψ ∈ usable_clauses ?A ?δ ∧ _ ] =>
+        assert (using_binary (root t1) (root t2) φ (length (word t1)) ∈ usable_clauses A δ) by
+          (apply elem_of_usable_clauses; split; [done 
+            | erewrite <-slice_length; [ eapply app_length_le_l; eauto | by rewrite decode_length ]
+          ]);
+        eexists; split; [eauto|]; wrap H
       end.
       all: split; first try congruence.
       12: {
@@ -479,106 +608,66 @@ Section encoding.
         have Hw : word t1_1 ++ word t1_2 = word t2_1 ++ word t2_2 by congruence.
         apply app_inj_1 in Hw => //. naive_solver.
       }
-      all: try (split; eapply Φ_pro_witness; simpl; eauto).
+      all: try (split; eapply Φ_using_derive_witness; simpl; eauto).
       all: repeat match goal with
       | [ |- _ ▷ _ ={ _ }=> _ ] =>
         repeat split; simpl; try done; try congruence; econstructor; eauto
-      | [ H : [] = decode _ _ ?δ |- ?δ = 0 ∧ _ ] =>
-        symmetry in H; rewrite H; apply decode_empty in H;
-        split; first done
-      | [ H : [_] = decode _ _ ?δ |- ?δ = 1 ∧ _ = term _ _ ∧ _ ] =>
-        symmetry in H; rewrite H; apply decode_singleton in H as [? [? ?]];
-        do 2 (split; first done)
-      | [ |- word ?t = decode _ _ _ ∧ _ ] =>
-        split; first by erewrite decode_app_l; eauto
+      | [ H : [] = slice (decode _ _) _ ?δ |- ?δ = 0 ∧ _ ] =>
+        rewrite -H; symmetry in H; apply slice_nil_iff in H; [|by rewrite decode_length]; split; first done
+      | [ H : [_] = slice (decode _ _) _ ?δ |- ?δ = 1 ∧ _ = term _ _ ∧ _ ] =>
+        rewrite -H; symmetry in H; apply slice_singleton_iff in H;
+        let H' := fresh in destruct H as [-> H']; rewrite decode_lookup in H'; [lia|];
+        inversion H'; subst; clear H'; do 2 (split; first done)
       | [ |- ∃ t, root t = root ?t' ∧ _ ] =>
         exists t'; split; first done
       | [ |- ∃ t1 t2, root t1 = root ?t1' ∧ root t2 = root ?t2' ∧ _ ] =>
         exists t1', t2'; do 2 (split; first done)
+      | [ |- word ?t = slice (decode _ _) _ _ ∧ _ ] =>
+        split; first by eapply slice_app_inv_NoDup_l; eauto
       end.
-  Qed.
+  Admitted.
 
   (* Main theorems *)
 
-  Definition Φ_amb A k : formula := λ m,
-    Φ_derive k m ∧ Φ_reach k A m ∧ ∃ H x δ, x + δ ≤ k ∧
-      can_reach_from m H x δ = true ∧ Φ_multi H x δ m.
+  Definition Φ_amb A : formula := λ k m,
+    Φ_derive k m ∧ Φ_reach A k m ∧ ∃ H,
+     (ε_can_reach_from m H = true ∧ Φ_multi_usable H 0 0 k m) ∨
+     (∃ x δ, 0 < δ ∧ x + δ ≤ k ∧ can_reach_from m H x δ = true ∧ Φ_multi_usable H x δ k m).
 
   Theorem Φ_amb_sound A k m :
-    Φ_amb A k m → derive_amb G A (decode m 0 k).
-  Admitted.
-
-  Variable error_letter : Σ.
-  Implicit Type w : sentence Σ.
-
-  Fixpoint slice w x δ : sentence Σ :=
-    match δ with
-    | 0 => []
-    | S n =>
-      match w !! x with
-      | Some tk => tk :: slice w (x + 1) n
-      | None => []
-      end
-    end.
-
-  (* TODO: why this instance cannot be found? *)
-  (* Check acyclic_derive_dec. *)
-  (* Check acyclic_reachable_dec. *)
-
-  Global Instance acyclic_derive_dec A w :
-    Decision (G ⊨ A ⇒ w).
-  Admitted.
-
-  Global Instance acyclic_reachable_dec A w H h :
-    Decision (reachable G (A, w) (H, h)).
-  Admitted.
-
-  Definition encode (w : sentence Σ) S : model := {|
-    term i :=
-      match w !! i with
-      | Some (a @ _) => a
-      | None => error_letter
-      end;
-    line i :=
-      match w !! i with
-      | Some (_ @ (x, _)) => x
-      | None => 0
-      end;
-    col i :=
-      match w !! i with
-      | Some (_ @ (_, y)) => y
-      | None => 0
-      end;
-    can_derive A x δ := bool_decide (G ⊨ A ⇒ (slice w x δ));
-    can_reach_from A x δ := bool_decide (reachable G (S, w) (A, slice w x δ));
-  |}.
-
-  Lemma reachable_sub_word A w H h :
-    reachable G (A, w) (H, h) →
-    ∃ w1 w2, w = w1 ++ h ++ w2.
-  Admitted.
-
-  Theorem Φ_amb_complete A k w :
-    length w = k →
-    derive_amb G A w →
-    ∃ m, Φ_amb A k m (* ∧ decode m 0 k = w *).
+    Φ_amb A k m → derive_amb G A (decode m k).
   Proof.
-    intros Hk Hamb.
+    intros [? [[? ?] [X HX]]].
+    apply derive_amb_iff_local_amb => //.
+    destruct HX as [[? Hm]|[x [δ [? [? [? Hm]]]]]].
+    - exists X, []; split; first by apply Φ_reach_empty_spec.
+      eapply Φ_multi_usable_spec in Hm; eauto; last lia.
+      simpl in Hm. naive_solver.
+    - exists X, (slice (decode m k) x δ); split; first by apply Φ_reach_nonempty_spec.
+      eapply Φ_multi_usable_spec in Hm; eauto. naive_solver.
+  Qed.
+
+  Theorem Φ_amb_complete X k w :
+    length w = k → derive_amb G X w → ∃ m, Φ_amb X k m.
+  Proof.
+    intros <- Hamb.
     apply derive_amb_iff_local_amb in Hamb; eauto.
-    destruct Hamb as [H [h [Hr [t1 [t2 [Ht1 [Ht2 Hne]]]]]]].
-    exists (encode w A).
-    have HΦ : Φ_derive k (encode w A).
-    { intros ?????. simpl. rewrite !bool_decide_eq_true. admit. }
-    have HΦ' : Φ_reach k A (encode w A).
-    { intros ????. simpl. rewrite !bool_decide_eq_true. admit. }
-    split => //. split => //.
-    have Hr' := Hr.
-    apply reachable_sub_word in Hr' as [w1 [w2 Hw]].
-    exists H, (length w1), (length h).
-    have ? : length w1 + length h ≤ k by admit.
-    split => //.
-    split. rewrite bool_decide_eq_true. admit. (* slice lemma *)
-    admit. (* multi_derive_encoding complete *)
-  Admitted.
+    destruct Hamb as [C [h [Hr [t1 [t2 [Ht1 [Ht2 Hne]]]]]]].
+    exists (encode X w).
+    have HΦ : Φ_derive (length w) (encode X w) by apply Φ_derive_sat.
+    have HΦ' : Φ_reach X (length w) (encode X w) by apply Φ_reach_sat.
+    do 2 (split; first done). exists C.
+    destruct h as [|tk h].
+    - left. rewrite bool_decide_eq_true. split; first done.
+      eapply Φ_multi_usable_spec; eauto; lia.
+    - right.
+      have Hsub : sublist (tk :: h) w by eapply reachable_sublist; eauto.
+      apply sublist_slice in Hsub as [x [? Hh]].
+      exists x, (length (tk :: h)).
+      rewrite bool_decide_eq_true -Hh. repeat split => //.
+      1: rewrite cons_length; lia.
+      eapply Φ_multi_usable_spec; eauto; try congruence.
+      rewrite decode_encode -Hh; eauto.
+  Qed.
 
 End encoding.
