theories/derivation.v
@@ -1,0 +1,84 @@
+From stdpp Require Import relations list.
+From Coq Require Import ssreflect.
+From ambig Require Import grammar.
+
+Section derivation.
+
+  Context {Σ N : Type} `{EqDecision Σ} `{EqDecision N}.
+  Context (G : grammar Σ N).
+
+  Inductive derivation : N → sentence Σ → Prop :=
+  | derive_ε A :
+    A ↦ ε ∈ G →
+    derivation A []
+  | derive_atom A a p :
+    A ↦ atom a ∈ G →
+    derivation A [a @ p]
+  | derive_unary A B φ w :
+    A ↦ unary B φ ∈ G →
+    apply₁ φ w = true →
+    derivation B w →
+    derivation A w
+  | derive_binary A Bl Br φ w1 w2 :
+    A ↦ binary Bl Br φ ∈ G →
+    apply₂ φ w1 w2 = true →
+    derivation Bl w1 →
+    derivation Br w2 →
+    derivation A (w1 ++ w2)
+  .
+
+  Lemma derivation_spec A w :
+    derivation A w ↔ G ⊨ A ⇒ w.
+  Proof.
+    split.
+    - (* -> *)
+      induction 1.
+      + exists (ε_tree A).
+        repeat split. by constructor.
+      + exists (token_tree A (a @ p)).
+        repeat split. by constructor.
+      + destruct IHderivation as [t [? [? ?]]].
+        exists (unary_tree A t).
+        repeat split => //=. econstructor; naive_solver.
+      + destruct IHderivation1 as [t1 [? [? ?]]].
+        destruct IHderivation2 as [t2 [? [? ?]]].
+        exists (binary_tree A t1 t2).
+        repeat split => //; try naive_solver.
+        econstructor; naive_solver.
+    - (* <- *)
+      intros [t [? [? Ht]]].
+      generalize dependent w.
+      generalize dependent A.
+      induction t; inversion Ht; subst => ????.
+      all: simpl in *; subst.
+      + by constructor.
+      + by constructor.
+      + eapply derive_unary; eauto.
+      + eapply derive_binary; eauto.
+  Qed.
+
+  Definition check_derive A w : Prop :=
+    (w = [] ∧ A ↦ ε ∈ G) ∨
+    (∃ a p, w = [a @ p] ∧ A ↦ atom a ∈ G) ∨
+    (∃ B φ, A ↦ unary B φ ∈ G ∧ apply₁ φ w = true ∧ derivation B w) ∨
+    (∃ Bl Br φ, A ↦ binary Bl Br φ ∈ G ∧ ∃ w1 w2, w = w1 ++ w2 ∧
+      apply₂ φ w1 w2 = true ∧ derivation Bl w1 ∧ derivation Br w2)
+    .
+
+  Lemma check_derive_spec A w :
+    check_derive A w ↔ derivation A w.
+  Proof.
+    split.
+    - intros [H|[H|[H|H]]].
+      + destruct H as [-> ?]. by constructor.
+      + destruct H as [a [p [-> ?]]]. by constructor.
+      + destruct H as [B [φ [? [? ?]]]]. eapply derive_unary; eauto.
+      + destruct H as [Bl [Br [φ [? [w1 [w2 [-> [? [? ?]]]]]]]]]. eapply derive_binary; eauto.
+    - inversion 1; subst.
+      + by left.
+      + right; left. naive_solver.
+      + right; right; left. naive_solver.
+      + right; right; right. naive_solver.
+  Qed.
+
+End derivation.
