theories/witness.v
@@ -1,0 +1,32 @@
+From stdpp Require Import relations list.
+From Coq Require Import ssreflect.
+From ambig Require Import grammar.
+
+Section witness.
+
+  Context {Σ N : Type} `{EqDecision Σ} `{EqDecision N}.
+  Context (G : grammar Σ N).
+
+  Lemma witness_ε A :
+    A ↦ ε ∈ G →
+    ε_tree A ▷ A ={ G }=> [].
+  Admitted.
+
+  Lemma witness_atom A a p :
+    A ↦ atom a ∈ G →
+    token_tree A (a @ p) ▷ A ={ G }=> [a @ p].
+  Admitted.
+
+  Lemma witness_unary A B φ t w :
+    A ↦ unary B φ ∈ G →
+    unary_tree A t ▷ A ={G}=> w ↔
+    t ▷ B ={G}=> w ∧ apply₁ φ w = true.
+  Admitted.
+
+  Lemma witness_binary A Bl Br φ t1 t2 w1 w2 :
+    A ↦ binary Bl Br φ ∈ G →
+    binary_tree A t1 t2 ▷ A ={G}=> (w1 ++ w2) ↔
+    t1 ▷ Bl ={G}=> w1 ∧ t2 ▷ Br ={G}=> w2 ∧ apply₂ φ w1 w2 = true.
+  Admitted.
+
+End witness.
